Solved HW 9

lean/love09_hoare_logic_homework_sheet.lean
@@ -70,33 +70,59 @@ namespace partial_hoare
 lemma consequence {P P' Q Q' : state → Prop} {S} (h : {* P *} S {* Q *})
     (hp : ∀s, P' s → P s) (hq : ∀s, Q s → Q' s) :
   {* P' *} S {* Q' *} :=
-sorry
+begin
+  intros s t hs' hst,
+  apply hq t,
+  apply h s t,
+  { exact hp s hs', },
+  { exact hst, }
+end
 
 /-! 1.2 (1 point). Prove the rule for `assign`. -/
 
 lemma assign_intro {P : state → Prop} {x} {a : state → ℕ} :
   {* λs, P (s{x ↦ a s}) *} stmt.assign x a {* P *} :=
-sorry
+begin
+  intros s t hs hst,
+  cases' hst, exact hs,
+end
 
 /-! 1.3 (1 point). Prove the rule for `seq`. -/
 
 lemma seq_intro {P Q R S T} (hS : {* P *} S {* Q *}) (hT : {* Q *} T {* R *}) :
   {* P *} stmt.seq S T {* R *} :=
-sorry
+begin
+  intros s t hs hst,
+  cases' hst with _ _ _ _ _ _ r _ hsr hrt,
+  apply hT r t,
+  { apply hS s r; assumption, },
+  { exact hrt, }
+end
 
 /-! 1.4 (1 point). Prove the rule for `it`. -/
 
 lemma it_intro {b P Q : state → Prop} {S}
     (htrue : {* λs, P s ∧ b s *} S {* Q *}) (hfalse : ∀s, P s ∧ ¬ b s → Q s) :
   {* P *} stmt.it b S {* Q *} :=
-sorry
+begin
+  intros s t hs hst,
+  cases' hst,
+  { apply htrue s t; try { apply and.intro }; assumption, },
+  { apply hfalse t; try { apply and.intro }; assumption, }
+end
 
 /-! 1.5 (2 points). Prove the rule for `loop`. Notice the similarity with the
 rule for `while` in the WHILE language. -/
 
 lemma loop_intro {S} (P : state → Prop) (h : {* P *} S {* P *}) :
   {* P *} stmt.loop S {* P *} :=
-sorry
+begin
+  intros s t hs hst,
+  induction' hst,
+  { apply ih_hst_1 P h,
+    exact h _ _ hs hst, },
+  { exact hs, }
+end
 
 end partial_hoare
 
@@ -117,8 +143,9 @@ stmt.while (λs, s "n" ≠ 0)
 /-! 2.1 (1 point). Define a recursive function that computes 2 to the power of
 `n`. -/
 
-def two_to_the_nth : ℕ → ℕ :=
-sorry
+def two_to_the_nth : ℕ → ℕ
+| 0       := 1
+| (n + 1) := 2 * two_to_the_nth n
 
 /-! Remember to test your function. Otherwise, you will have big difficulties
 answering question 2.2 below. -/
@@ -133,6 +160,20 @@ answering question 2.2 below. -/
 
 lemma POWER_OF_TWO_correct (n₀ : ℕ) :
   {* λs, s "n" = n₀ *} POWER_OF_TWO {* λs, s "y" = two_to_the_nth n₀ *} :=
-sorry
+show {* λs, s "n" = n₀ *}
+     stmt.assign "y" (λs, 1) ;;
+     stmt.while_inv (λs, s "y" * two_to_the_nth (s "n") = two_to_the_nth n₀) (λs, s "n" ≠ 0)
+       (stmt.assign "y" (λs, s "y" * 2) ;;
+        stmt.assign "n" (λs, s "n" - 1))
+     {* λs, s "y" = two_to_the_nth n₀ *}, from
+  begin
+    vcg; intro s; simp,
+    { cases' s "n"; simp, intro h,
+      simp [←h, two_to_the_nth, mul_assoc], },
+    { intros h₁ h₂,
+      simp [h₁, two_to_the_nth] at h₂,
+      exact h₂, },
+    { intro h, rw h, }
+  end
 
 end LoVe
